proof: TM_to_GOTO_on_List_correct_and_in_linear_time'; TM_to_GOTO_on_List_correct_and_in_linear_time
fix:
statement of several lemmas that incorrectly stated conclusions concerning the same variable;
make configuration_of_prog_same_to_TM and wf_cfg definitions instead of abbreviations to make proof state more readable

todos:
prove extra properties about TM;
prove the correctness of each the 5 parts of the transformed GOTO_on_List program

IMPminus_TM/TM_GOTO/TM_to_GOTO_on_List.thy
@@ -183,23 +183,105 @@ qed
 abbreviation GOTO_on_List_Prog :: "GOTO\<^sub>l_prog" where
   "GOTO_on_List_Prog \<equiv> HALT\<^sub>l # entrance_block @ blocks_for_actions @ [HALT\<^sub>l]"
 
-subsection \<open>Correctness of the transform function\<close>
 
-abbreviation configuration_of_prog_same_to_TM :: "state\<^sub>l \<Rightarrow> config \<Rightarrow> bool" (\<open>_ \<sim> _\<close> 50) where
+subsection \<open>Properties about state and configuration and their preservation\<close>
+text \<open>The verification requires some properties about the state of the GOTO_on_List program,
+as well as the corresponding TM configuration. Below are some definitions and lemma about them
+and their preservation through execution.\<close>
+
+definition configuration_of_prog_same_to_TM :: "state\<^sub>l \<Rightarrow> config \<Rightarrow> bool" (\<open>_ \<sim> _\<close> 50) where
   "s \<sim> cfg \<equiv>
     s ST = [fst cfg] \<and> \<comment>\<open>state\<close>
     (\<forall>k < K. s (HP k) = [cfg <#> k]) \<and> \<comment>\<open>head positions of each tape\<close>
     (\<forall>k < K. \<forall>p < MAX_LEN. (s (TP k)) ! p = (cfg <:> k) p)" \<comment>\<open>tape content\<close>
 
-abbreviation wf_cfg :: "config \<Rightarrow> bool" where
+lemma configuration_of_prog_same_to_TM_D [intro]:
+  assumes "s \<sim> cfg"
+    shows "s ST = [fst cfg]"
+      and "\<forall>k < K. s (HP k) = [cfg <#> k]"
+      and "\<forall>k < K. \<forall>p < MAX_LEN. (s (TP k)) ! p = (cfg <:> k) p"
+  using assms configuration_of_prog_same_to_TM_def by simp_all
+
+lemma configuration_of_prog_same_to_TM_I:
+  assumes "s ST = [fst cfg]"
+      and "\<forall>k < K. s (HP k) = [cfg <#> k]"
+      and "\<forall>k < K. \<forall>p < MAX_LEN. (s (TP k)) ! p = (cfg <:> k) p"
+    shows "s \<sim> cfg"
+  unfolding configuration_of_prog_same_to_TM_def
+  using assms by blast
+
+definition wf_cfg :: "config \<Rightarrow> bool" where
   "wf_cfg cfg \<equiv>
     fst cfg \<le> Q \<and> \<comment>\<open>state, = Q means halting state\<close>
-    length (snd cfg) = K \<and> \<comment>\<open>number of tapes\<close>
+    ||cfg|| = K \<and> \<comment>\<open>number of tapes\<close>
     (\<forall>k < K. \<forall>p < MAX_LEN. (cfg <:> k) p < G) \<and> \<comment>\<open>tape content consists of characters < G only\<close>
     (\<forall>k < K. cfg <#> k < MAX_LEN)" \<comment>\<open>tape head position not exceeding max used length of tape\<close>
 
+lemma wf_cfg_D [intro]:
+  assumes "wf_cfg cfg"
+    shows "fst cfg \<le> Q"
+      and "||cfg|| = K"
+      and "\<forall>k < K. \<forall>p < MAX_LEN. (cfg <:> k) p < G"
+      and "\<forall>k < K. cfg <#> k < MAX_LEN"
+  using assms wf_cfg_def by simp_all
+
+lemma wf_cfg_I:
+  assumes "fst cfg \<le> Q"
+      and "||cfg|| = K"
+      and "\<forall>k < K. \<forall>p < MAX_LEN. (cfg <:> k) p < G"
+      and "\<forall>k < K. cfg <#> k < MAX_LEN"
+    shows "wf_cfg cfg"
+  unfolding wf_cfg_def
+  using assms by blast
+
 lemma wf_cfg_start_cfg: "wf_cfg (0, TPS)"
-  using wf_TPS by simp
+  using wf_TPS
+  by (simp add: wf_cfg_def)
+
+lemma wf_cfg_preserved_by_exe [intro]:
+  assumes "wf_cfg cfg"
+      and "exe M cfg = cfg'"
+    shows "wf_cfg cfg'"
+proof (cases "fst cfg < Q")
+  case True
+  with TM Q have "turing_command K Q G (M ! fst cfg)"
+    by (simp add: turing_machineD(3))
+  from \<open>exe M cfg = cfg'\<close> True have "cfg' = sem (M ! fst cfg) cfg"
+    by (simp add: Q exe_lt_length)
+    
+  have "fst cfg' \<le> Q" sorry
+  moreover
+  have "||cfg'|| = K" sorry
+  moreover
+  have "\<forall>k<K. \<forall>p<MAX_LEN. (cfg' <:> k) p < G"
+  proof(standard; standard; standard; standard)
+    fix k p assume "k < K" "p < MAX_LEN"
+    then show "(cfg' <:> k) p < G" sorry
+  qed
+  moreover
+  have "\<forall>k<K. cfg' <#> k < MAX_LEN"
+  proof (standard; standard)
+    fix k assume "k < K"
+    then show "cfg' <#> k < MAX_LEN" sorry
+  qed
+  ultimately
+  show ?thesis by (simp add: wf_cfg_I)
+next
+  case False
+  with \<open>wf_cfg cfg\<close> have "fst cfg = Q"
+    using le_neq_implies_less by blast
+  with \<open>exe M cfg = cfg'\<close> have "cfg' = cfg"
+    by (simp add: Q exe_ge_length)
+  with \<open>wf_cfg cfg\<close> show ?thesis by force
+qed
+
+lemma wf_cfg_preserved_by_execute [intro]:
+  assumes "wf_cfg cfg"
+      and "execute M cfg t = cfg'"
+    shows "wf_cfg cfg'"
+  using assms
+  by (induction t arbitrary: cfg') auto
+
 
 abbreviation read_chars_correspond_to_cfg :: "state\<^sub>l \<Rightarrow> config \<Rightarrow> bool" where
   "read_chars_correspond_to_cfg s cfg \<equiv> (\<forall>k < K. s CHS ! k = cfg <.> k) \<and> length (s CHS) = K"
@@ -228,9 +310,10 @@ next
 qed
 
 lemma config_to_state_correct [simp]: "config_to_state cfg \<sim> cfg"
-  using tape_content_to_list_correct
+  using tape_content_to_list_correct configuration_of_prog_same_to_TM_I
   by (metis config_to_state.simps(1-3) surjective_pairing)
 
+subsection \<open>Correctness of the transform function\<close>
 text \<open>Each step in the Turing Machine corresponds to no more than
 (entrance_block_len + block_for_q_chs_len) steps in the transformed GOTO_on_List program,
 starting from pc = 1, ending also at pc = 1.
@@ -253,7 +336,8 @@ lemma read_state_and_chars_correct:
   assumes "wf_cfg cfg"
       and "s \<sim> cfg"
       and "fst cfg < Q" \<comment>\<open>not in halting state\<close>
-    shows "GOTO_on_List_Prog \<turnstile>\<^sub>l (pc_start, s) \<rightarrow>\<^bsub>2\<^esub> (pc_start + 2, s')"
+  obtains s'
+    where "GOTO_on_List_Prog \<turnstile>\<^sub>l (pc_start, s) \<rightarrow>\<^bsub>2\<^esub> (pc_start + 2, s')"
       and "s' \<sim> cfg"
       and "read_chars_correspond_to_cfg s' cfg"
   sorry
@@ -281,11 +365,11 @@ lemma block_for_q_chs_correct:
       and "s \<sim> cfg"
       and "read_chars_correspond_to_cfg s cfg"
       and "exe M cfg = cfg'"
-    shows "GOTO_on_List_Prog \<turnstile>\<^sub>l
+  obtains s'
+    where "GOTO_on_List_Prog \<turnstile>\<^sub>l
            (label_of_block_for_q_chs (hd (s ST), s CHS), s) \<rightarrow>\<^bsub>block_for_q_chs_len\<^esub>
            (label_of_block_for_q_chs (hd (s ST), s CHS) + block_for_q_chs_len, s')"
       and "s' \<sim> cfg'"
-      and "wf_cfg cfg'"
   sorry
 
 lemma jump_back_to_begin:
@@ -298,20 +382,19 @@ corollary TM_to_GOTO_on_List_correct_for_single_step:
   assumes "wf_cfg cfg"
       and "fst cfg < Q"
       and "exe M cfg = cfg'"
-  obtains s
+      and "s \<sim> cfg"
+  obtains s'
     where "\<exists>t_entrance \<le> entrance_block_len.
            GOTO_on_List_Prog \<turnstile>\<^sub>l
-           (pc_start, config_to_state cfg)
+           (pc_start, s)
            \<rightarrow>\<^bsub>t_entrance + block_for_q_chs_len + 2\<^esub>
-           (pc_start, s)"
-      and "s \<sim> cfg'"
-      and "wf_cfg cfg'"
+           (pc_start, s')"
+      and "s' \<sim> cfg'"
 proof -
-  have "config_to_state cfg \<sim> cfg" by simp
-  with \<open>wf_cfg cfg\<close> \<open>fst cfg < Q\<close> obtain s\<^sub>1 where read_state_and_chars_correct:
-    "GOTO_on_List_Prog \<turnstile>\<^sub>l (pc_start, config_to_state cfg) \<rightarrow>\<^bsub>2\<^esub> (pc_start + 2, s\<^sub>1)"
+  from \<open>wf_cfg cfg\<close> \<open>fst cfg < Q\<close> \<open>s \<sim> cfg\<close> obtain s\<^sub>1 where read_state_and_chars_correct:
+    "GOTO_on_List_Prog \<turnstile>\<^sub>l (pc_start, s) \<rightarrow>\<^bsub>2\<^esub> (pc_start + 2, s\<^sub>1)"
     and s\<^sub>1: "s\<^sub>1 \<sim> cfg" "read_chars_correspond_to_cfg s\<^sub>1 cfg"
-    using read_state_and_chars_correct [where ?s = "config_to_state cfg"] by presburger
+    using read_state_and_chars_correct by blast
   with \<open>wf_cfg cfg\<close> have search_for_correct_label_for_q_and_chs:
     "GOTO_on_List_Prog \<turnstile>\<^sub>l
      (pc_start + 2, s\<^sub>1) \<rightarrow>\<^bsub>index q_chs_enum_list (hd (s\<^sub>1 ST), s\<^sub>1 CHS)\<^esub>
@@ -326,7 +409,7 @@ proof -
     "GOTO_on_List_Prog \<turnstile>\<^sub>l
      (label_of_block_for_q_chs (hd (s\<^sub>1 ST), s\<^sub>1 CHS), s\<^sub>1) \<rightarrow>\<^bsub>block_for_q_chs_len\<^esub>
      (label_of_block_for_q_chs (hd (s\<^sub>1 ST), s\<^sub>1 CHS) + block_for_q_chs_len, s\<^sub>2)"
-    and "s\<^sub>2 \<sim> cfg'" and "wf_cfg cfg'"
+    and "s\<^sub>2 \<sim> cfg'"
     using block_for_q_chs_correct [where ?s = s\<^sub>1 and ?cfg = cfg and ?cfg' = cfg']
     by blast
   have jump_back_to_begin:
@@ -336,16 +419,18 @@ proof -
     using jump_back_to_begin by blast
 
   from read_state_and_chars_correct search_for_correct_label_for_q_and_chs
-  have "GOTO_on_List_Prog \<turnstile>\<^sub>l (pc_start, config_to_state cfg)
+  have "GOTO_on_List_Prog \<turnstile>\<^sub>l (pc_start, s)
         \<rightarrow>\<^bsub>2 + index q_chs_enum_list (hd (s\<^sub>1 ST), s\<^sub>1 CHS)\<^esub>
         (pc_start + 2 + index q_chs_enum_list (hd (s\<^sub>1 ST), s\<^sub>1 CHS), s\<^sub>1)"
     by blast
   moreover
   have "(hd (s\<^sub>1 ST), s\<^sub>1 CHS) \<in> set q_chs_enum_list"
   proof -
-    from \<open>s\<^sub>1 \<sim> cfg\<close> \<open>fst cfg < Q\<close> \<open>wf_cfg cfg\<close> have "hd (s\<^sub>1 ST) < Q" by auto
+    from \<open>s\<^sub>1 \<sim> cfg\<close> \<open>fst cfg < Q\<close> \<open>wf_cfg cfg\<close> have "hd (s\<^sub>1 ST) < Q"
+      by (simp add: configuration_of_prog_same_to_TM_D(1))
     
-    from s\<^sub>1 \<open>s\<^sub>1 \<sim> cfg\<close> \<open>wf_cfg cfg\<close> have "\<forall>k<K. s\<^sub>1 CHS ! k < G" by simp
+    from s\<^sub>1 \<open>s\<^sub>1 \<sim> cfg\<close> \<open>wf_cfg cfg\<close> have "\<forall>k<K. s\<^sub>1 CHS ! k < G"
+      by (simp add: wf_cfg_D(3) wf_cfg_D(4))
     then have "\<forall>k<K. s\<^sub>1 CHS ! k \<in> set [0..<G]" by simp
     moreover
     from s\<^sub>1 have "length (s\<^sub>1 CHS) = K" by blast
@@ -357,78 +442,145 @@ proof -
     using q_chs_enum_list_length by fastforce
   ultimately
   obtain t_entrance where "t_entrance \<le> entrance_block_len" and
-    "GOTO_on_List_Prog \<turnstile>\<^sub>l (pc_start, config_to_state cfg) \<rightarrow>\<^bsub>t_entrance\<^esub>
+    "GOTO_on_List_Prog \<turnstile>\<^sub>l (pc_start, s) \<rightarrow>\<^bsub>t_entrance\<^esub>
      (pc_start + 2 + index q_chs_enum_list (hd (s\<^sub>1 ST), s\<^sub>1 CHS), s\<^sub>1)"
     using entrance_block_length
     by (metis (no_types, lifting) add_2_eq_Suc less_imp_le_nat nat_add_left_cancel_le)
   with jump_to_correct_label
-  have "GOTO_on_List_Prog \<turnstile>\<^sub>l (pc_start, config_to_state cfg) \<rightarrow>\<^bsub>t_entrance + 1\<^esub>
+  have "GOTO_on_List_Prog \<turnstile>\<^sub>l (pc_start, s) \<rightarrow>\<^bsub>t_entrance + 1\<^esub>
         (label_of_block_for_q_chs (hd (s\<^sub>1 ST), s\<^sub>1 CHS), s\<^sub>1)"
     by auto        
   with block_for_q_chs_correct
-  have "GOTO_on_List_Prog \<turnstile>\<^sub>l (pc_start, config_to_state cfg)
+  have "GOTO_on_List_Prog \<turnstile>\<^sub>l (pc_start, s)
         \<rightarrow>\<^bsub>t_entrance + 1 + block_for_q_chs_len\<^esub>
         (label_of_block_for_q_chs (hd (s\<^sub>1 ST), s\<^sub>1 CHS) + block_for_q_chs_len, s\<^sub>2)"
     by blast
   with jump_back_to_begin
-  have "GOTO_on_List_Prog \<turnstile>\<^sub>l (pc_start, config_to_state cfg)
+  have "GOTO_on_List_Prog \<turnstile>\<^sub>l (pc_start, s)
         \<rightarrow>\<^bsub>t_entrance + 1 + block_for_q_chs_len + 1\<^esub>
         (pc_start, s\<^sub>2)"
     by auto
 
   with \<open>t_entrance \<le> entrance_block_len\<close>
   have "\<exists>t_entrance \<le> entrance_block_len.
-         GOTO_on_List_Prog \<turnstile>\<^sub>l  (pc_start, config_to_state cfg)
+         GOTO_on_List_Prog \<turnstile>\<^sub>l  (pc_start, s)
          \<rightarrow>\<^bsub>t_entrance + block_for_q_chs_len + 2\<^esub>
          (pc_start, s\<^sub>2)" by auto
-  with \<open>s\<^sub>2 \<sim> cfg'\<close> \<open>wf_cfg cfg'\<close>
+  with \<open>s\<^sub>2 \<sim> cfg'\<close>
   show thesis using that by presburger
-qed
-    
-lemma prog_correctly_ends:
-  "GOTO_on_List_Prog \<turnstile>\<^sub>l
-   (pc_start, config_to_state (Q, tps)) \<rightarrow>\<^bsub>1\<^esub> (pc_halt, config_to_state (Q, tps))"
-proof -
-  have "config_to_state (Q, tps) ST = [Q]"
-    by fastforce
-  have "iexec\<^sub>l (IF ST = L [Q] THEN GOTO\<^sub>l pc_halt) (pc, config_to_state (Q, tps)) =
-        (pc_halt, config_to_state (Q, tps))" for pc
-    by simp
-  then have "GOTO_on_List_Prog \<turnstile>\<^sub>l
-    (pc_start, config_to_state (Q, tps)) \<rightarrow> (pc_halt, config_to_state (Q, tps))"
-    by force
-  then show ?thesis by auto
 qed
 
 lemma TM_to_GOTO_on_List_correct_and_in_linear_time':
-  assumes "s \<sim> cfg"
+  assumes "s = config_to_state cfg"
+      and "wf_cfg cfg"
+      and "fst cfg < Q"
       and "execute M cfg t = cfg'"
-    shows "\<exists>c. \<exists>t' \<le> c * t.
-          (GOTO_on_List_Prog \<turnstile>\<^sub>l (pc_start, s) \<rightarrow>\<^bsub>t'\<^esub> (pc_halt, s'))"
-      and "s' \<sim> cfg'"
+    shows "\<exists>s'. (s' \<sim> cfg') \<and>
+          (\<exists>t' \<le> (entrance_block_len + block_for_q_chs_len + 2) * t.
+           GOTO_on_List_Prog \<turnstile>\<^sub>l (pc_start, s) \<rightarrow>\<^bsub>t'\<^esub> (pc_start, s'))"
   using assms
-   apply (induction t)
-  sorry
+proof (induction t arbitrary: cfg')
+  case 0
+  then show ?case by auto
+next
+  case (Suc t)
+  from \<open>execute M cfg (Suc t) = cfg'\<close> obtain cfg_mid where cfg_mid:
+    "execute M cfg t = cfg_mid" "exe M cfg_mid = cfg'"
+    by auto
+  with \<open>wf_cfg cfg\<close> have "wf_cfg cfg_mid" by blast
+  with cfg_mid Suc.IH assms obtain t' s_mid where
+    t': "t' \<le> (entrance_block_len + block_for_q_chs_len + 2) * t" and
+    s_mid: "GOTO_on_List_Prog \<turnstile>\<^sub>l (pc_start, s) \<rightarrow>\<^bsub>t'\<^esub> (pc_start, s_mid)" "s_mid \<sim> cfg_mid"
+    by auto
+  show ?case
+  proof (cases "fst cfg_mid < Q")
+    case True
+    with \<open>exe M cfg_mid = cfg'\<close> \<open>wf_cfg cfg_mid\<close> \<open>s_mid \<sim> cfg_mid\<close>
+    obtain s' where
+      "\<exists>t_entrance\<le>entrance_block_len.
+        GOTO_on_List_Prog
+        \<turnstile>\<^sub>l (pc_start, s_mid) \<rightarrow>\<^bsub>t_entrance + block_for_q_chs_len + 2\<^esub> (pc_start, s')"
+      "s' \<sim> cfg'"
+      using TM_to_GOTO_on_List_correct_for_single_step
+      by blast
+    then obtain t_last_step where
+      t_last_step: "t_last_step \<le> entrance_block_len + block_for_q_chs_len + 2" and
+      s': "GOTO_on_List_Prog \<turnstile>\<^sub>l (pc_start, s_mid) \<rightarrow>\<^bsub>t_last_step\<^esub> (pc_start, s')"
+      by (meson add_le_mono1)
+
+    with s_mid have "GOTO_on_List_Prog \<turnstile>\<^sub>l (pc_start, s) \<rightarrow>\<^bsub>t' + t_last_step\<^esub> (pc_start, s')"
+      by blast
+    moreover
+    from t' t_last_step have "t' + t_last_step \<le> (entrance_block_len + block_for_q_chs_len + 2) * (Suc t)"
+      by force
+    ultimately
+    show ?thesis using \<open>s' \<sim> cfg'\<close> by blast
+  next
+    case False
+    with \<open>exe M cfg_mid = cfg'\<close> Q have "cfg_mid = cfg'"
+      by (simp add: exe_ge_length)
+    moreover
+    from t' s_mid
+    have "t' \<le> (entrance_block_len + block_for_q_chs_len + 2) * Suc t \<and>
+          GOTO_on_List_Prog \<turnstile>\<^sub>l (pc_start, s) \<rightarrow>\<^bsub>t'\<^esub> (pc_start, s_mid)"
+      by auto
+    ultimately
+    show ?thesis
+      using s_mid by blast 
+  qed
+qed
+
 
 theorem TM_to_GOTO_on_List_correct_and_in_linear_time:
-  assumes "s \<sim> (0, TPS)"
-    shows "\<exists>t \<le> T. \<exists>c. \<exists>t' \<le> c * t.
-          (GOTO_on_List_Prog \<turnstile>\<^sub>l (pc_start, s) \<rightarrow>\<^bsub>t'\<^esub> (pc_halt, s'))"
-      and "s' \<sim> (Q, TPS')"
+  obtains s
+    where "\<exists>t \<le> T. \<exists>c. \<exists>t' \<le> c * t + 1.
+          (GOTO_on_List_Prog \<turnstile>\<^sub>l (pc_start, s\<^sub>0) \<rightarrow>\<^bsub>t'\<^esub> (pc_halt, s))"
+      and "s \<sim> (Q, TPS')"
 proof -
-  from runtime_M have execute_M: "\<exists>t \<le> T. execute M (0, TPS) t = (Q, TPS')"
+  from runtime_M obtain t where execute_M: "execute M (0, TPS) t = (Q, TPS')" and t: "t \<le> T"
     using Q unfolding transforms_def transits_def
-    by simp
-  with assms show
-    "\<exists>t \<le> T. \<exists>c. \<exists>t' \<le> c * t.
-     (GOTO_on_List_Prog \<turnstile>\<^sub>l (pc_start, s) \<rightarrow>\<^bsub>t'\<^esub> (pc_halt, s'))"
-    using TM_to_GOTO_on_List_correct_and_in_linear_time'
-    by (smt (verit, del_insts)
-        append1_eq_conv append_assoc concat_map_singleton config_to_state.simps(2) list.inject)
-  
-  from assms execute_M
-  show "s' \<sim> (Q, TPS')"
-    using TM_to_GOTO_on_List_correct_and_in_linear_time'(2) by blast
+    by blast
+  then obtain s t' where
+    "s \<sim> (Q, TPS')"
+    "t' \<le> (entrance_block_len + block_for_q_chs_len + 2) * t"
+    "GOTO_on_List_Prog \<turnstile>\<^sub>l (pc_start, s\<^sub>0) \<rightarrow>\<^bsub>t'\<^esub> (pc_start, s)"
+  proof (cases "Q = 0")
+    case True
+    with execute_M Q have "TPS' = TPS"
+      by (metis execute.simps(1) fst_conv halting_config_execute old.prod.inject) 
+    with \<open>Q = 0\<close> have "s\<^sub>0 \<sim> (Q, TPS')" by auto
+    moreover
+    have "GOTO_on_List_Prog \<turnstile>\<^sub>l (pc_start, s\<^sub>0) \<rightarrow>\<^bsub>0\<^esub> (pc_start, s\<^sub>0)"
+         "0 \<le> (entrance_block_len + block_for_q_chs_len + 2) * t"
+      by auto
+    ultimately
+    show ?thesis using that by blast 
+  next
+    case False
+    let ?cfg = "(0, TPS)"
+    from \<open>Q \<noteq> 0\<close> have "fst ?cfg < Q" by simp
+    moreover
+    from wf_cfg_start_cfg have "wf_cfg ?cfg" by simp
+    ultimately
+    show ?thesis
+      using execute_M
+      using TM_to_GOTO_on_List_correct_and_in_linear_time'
+            [where ?cfg = ?cfg and ?s = s\<^sub>0 and ?t = t and ?cfg' = "(Q, TPS')"]
+      using that by blast
+  qed
+  moreover
+  from \<open>s \<sim> (Q, TPS')\<close> have "GOTO_on_List_Prog \<turnstile>\<^sub>l (pc_start, s) \<rightarrow> (pc_halt, s)"
+    by fastforce
+  ultimately
+  have "\<exists>t' \<le> (entrance_block_len + block_for_q_chs_len + 2) * t + 1.
+        GOTO_on_List_Prog \<turnstile>\<^sub>l (pc_start, s\<^sub>0) \<rightarrow>\<^bsub>t'\<^esub> (pc_halt, s)"
+    by fastforce
+  then have "\<exists>c. \<exists>t' \<le> c * t + 1. GOTO_on_List_Prog \<turnstile>\<^sub>l (pc_start, s\<^sub>0) \<rightarrow>\<^bsub>t'\<^esub> (pc_halt, s)"
+    by fast
+  with t have "\<exists>t \<le> T. \<exists>c. \<exists>t' \<le> c * t + 1. GOTO_on_List_Prog \<turnstile>\<^sub>l (pc_start, s\<^sub>0) \<rightarrow>\<^bsub>t'\<^esub> (pc_halt, s)"
+    by blast
+  with \<open>s \<sim> (Q, TPS')\<close> show thesis
+    using that by blast
 qed
 
 end
